src/Minimal.DICE.fst
@@ -1,0 +1,81 @@
+/// Reference: https://github.com/microsoft/RIoT/blob/master/Reference/DICE/DiceCore.cpp
+module Minimal.DICE
+
+open LowStar.BufferOps
+open Lib.IntTypes
+open FStar.Integers
+
+open Spec.Hash.Definitions
+open Hacl.Hash.Definitions
+
+module I  = FStar.Integers
+module HI  = Lib.IntTypes
+
+module SHA2= Hacl.Hash.SHA2
+
+module B   = LowStar.Buffer
+module M   = LowStar.Modifies
+module HS  = FStar.HyperStack
+module HST = FStar.HyperStack.ST
+
+let _DICE_ALG = SHA2_256
+let _DICE_UDS_LENGTH    = 0x20
+let _DICE_DIGEST_LENGTH: uint_32 = hash_len _DICE_ALG
+
+/// <><><><><><><><><><><><><><><><><><><><><><><><><><><><><><><><><><><>
+
+assume val get_UDS
+  (size: nat)
+: HST.St (b:B.buffer HI.uint8 {B.length b = size})
+
+assume val get_measurement
+  (alg: hash_alg)
+: HST.St (hash_t alg)
+
+assume val diceSHA256_2
+  (size1 : nat)
+  (data1: B.lbuffer HI.uint8 size1)
+  (size2 : nat)
+  (data2 : B.lbuffer HI.uint8 size2)
+  (digest: hash_t _DICE_ALG)
+: HST.St unit
+
+/// <><><><><><><><><><><><> DICE Core main funtion <><><><><><><><><><><>
+
+#reset-options "--z3rlimit 10"
+let diceStart ()
+: HST.Stack (B.lbuffer uint8 (v _DICE_DIGEST_LENGTH))
+  (requires fun _ -> True)
+  (ensures  fun _ _ _ -> True)
+=
+  HST.push_frame();
+
+/// NOTE: compute digest `uDigest` of `uds`
+  let uds : B.lbuffer uint8 _DICE_UDS_LENGTH = get_UDS _DICE_UDS_LENGTH in
+  let uDigest :hash_t _DICE_ALG = B.alloca (HI.u8 0x00) _DICE_DIGEST_LENGTH in
+    SHA2.hash_256
+      uds
+      (u _DICE_UDS_LENGTH)
+      uDigest;
+
+/// NOTE: compute digest `rDigest` of `measurement`
+  let measurement: hash_t _DICE_ALG = get_measurement _DICE_ALG in
+  let rDigest :hash_t _DICE_ALG = B.alloca (HI.u8 0x00) _DICE_DIGEST_LENGTH in
+    SHA2.hash_256
+      measurement
+      _DICE_DIGEST_LENGTH
+      rDigest;
+
+    let cdi: hash_t _DICE_ALG
+      = B.alloca (HI.u8 0x00) _DICE_DIGEST_LENGTH in
+
+    diceSHA256_2
+     (v _DICE_DIGEST_LENGTH) uDigest
+     (v _DICE_DIGEST_LENGTH) rDigest
+     cdi;
+
+    B.fill uDigest (HI.u8 0x00) _DICE_DIGEST_LENGTH;
+    B.fill rDigest (HI.u8 0x00) _DICE_DIGEST_LENGTH;
+
+  HST.pop_frame();
+  cdi
