src/Minimal.Main.fst
@@ -1,0 +1,17 @@
+module Minimal.Main
+
+open Minimal.DICE
+open Minimal.RIoT
+
+module HST = FStar.HyperStack.ST
+
+let main ()
+: HST.Stack C.exit_code
+  (requires fun _ -> True)
+  (ensures  fun _ _ _ -> True)
+=
+  riotStart
+    Minimal.DICE._DICE_DIGEST_LENGTH
+    (diceStart ());
+
+  C.EXIT_SUCCESS
